Improve translation for set is singleton (#129)
* Refactor set is singleton

* Fix set is_singleton

Cpc/Spec.lean
@@ -387,8 +387,8 @@ def __eo_to_smt : Term -> SmtTerm
     let _v0 := (__eo_to_smt x1)
     (SmtTerm.eq _v0 (SmtTerm.set_empty (__smtx_typeof _v0)))
   | (Term.Apply (Term.UOp UserOp.set_is_singleton) x1) => 
-    let _v0 := (__eo_to_smt_type (__eo_typeof (Term.Apply (Term.UOp UserOp.set_choose) x1)))
-    (SmtTerm.exists "@x" _v0 (SmtTerm.eq (__eo_to_smt x1) (SmtTerm.set_singleton (SmtTerm.Var "@x" _v0))))
+    let _v0 := (__eo_to_smt x1)
+    (SmtTerm.eq _v0 (SmtTerm.set_singleton (SmtTerm.map_diff _v0 (SmtTerm.set_empty (__eo_to_smt_type (__eo_typeof (Term.Apply (Term.UOp UserOp.set_choose) x1)))))))
   | (Term.Apply (Term.Apply (Term.UOp UserOp.set_insert) Term.__eo_List_nil) x1) => SmtTerm.None
   | (Term.Apply (Term.Apply (Term.UOp UserOp.set_insert) x1) x2) => (__eo_to_smt_set_insert x1 (__eo_to_smt x2))
   | (Term.UOp2 UserOp2._at_sets_deq_diff x1 x2) => (native_ite (native_Teq (__eo_to_smt_type (Term.UOp2 UserOp2._at_sets_deq_diff x1 x2)) SmtType.None) SmtTerm.None (SmtTerm.map_diff (__eo_to_smt x1) (__eo_to_smt x2)))
